(a) Is $\circ$ associative on $S$?

Let's consider the given equation in (ii) and substitute $b = e$:

$$
\begin{aligned}
(a \circ b) \circ (c \circ d) & = (a \circ c) \circ (b \circ d) & \qquad \textrm{given} \\
(a \circ e) \circ (c \circ d) & = (a \circ c) \circ (e \circ d) & \qquad \textrm{substitute $b = e$} \\
a \circ (c \circ d) & = (a \circ c) \circ d & \qquad \textrm{given: $x \circ e = e \circ x = x$} \\
\end{aligned}
$$

This proves that $\boxed{\circ\ \text{is associative on} \ S.}$ $\quad \blacksquare$

Alternatively, we can set $c = e$ with similar results:

$$
\begin{aligned}
(a \circ b) \circ (c \circ d) & = (a \circ c) \circ (b \circ d) & \qquad \textrm{given} \\
(a \circ b) \circ (e \circ d) & = (a \circ e) \circ (b \circ d) & \qquad \textrm{substitute $c = e$} \\
(a \circ b) \circ d & = a \circ (b \circ d) & \qquad \textrm{given: $x \circ e = e \circ x = x$} \\
\end{aligned}
$$

This proves that $\boxed{\circ \ \text{is associative on} \ S.}$ $\quad \blacksquare$

However, we can't prove the same result if we set $a = e$ or $d = e$, why is
that? Exercise for the reader.

(b) Is $\circ$ commutative on $S$?

For this case, let's take the same given equation in (ii) and consider the case
where $a = e$ and $d = e$:

$$
\begin{aligned}
(a \circ b) \circ (c \circ d) & = (a \circ c) \circ (b \circ d) & \qquad \textrm{given} \\
(e \circ b) \circ (c \circ e) & = (e \circ c) \circ (b \circ e) &
    \qquad \textrm{substitute $a = e$, $d = e$} \\
b \circ c & = c \circ b & \qquad \textrm{given: $x \circ e = e \circ x = x$} \\
\end{aligned}
$$

This proves that $\boxed{\circ \ \text{is commutative on} \ S.}$ $\quad \blacksquare$
