The given sequence is already defined for us in the general case in the last
element:

$$ 1, (1 + 2), (1 + 2 + 2^2), ..., \textbf{$(1 + 2 + ... + 2^{k - 1})$}, ... $$

The $i^{th}$ term of this sequence can thus be written as follows:

$$ a_i = \sum_{i = 1}^{n} 2^{i-1} $$

Then, the sum of the first $n$ terms in the sequence is:

$$ \sum_{i = 1}^n a_i = \sum_{i = 1}^n \sum_{k = 1}^i 2^{k - 1} $$

However, we don't actually have to expand or simplify the double-summation.
Since we have $4$ unknowns, we can just compute the first $4$ values of $A_n$,
set them equal, and solve a system of $4$ equations with $4$ unknowns.

Let $A_n = \displaystyle{\sum_{i=1}^n a_i}$, and let's compute several of the
initial values:

$$
\begin{aligned}
A_1 & = a_1                   & = & \; 1                               & = & \;  1 \\
A_2 & = a_1 + a_2             & = & \; 1 + (1+2)                       & = & \;  4 \\
A_3 & = a_1 + a_2 + a_3       & = & \; 1 + (1+2) + (1+2+4)             & = & \; 11 \\
A_4 & = a_1 + a_2 + a_3 + a_4 & = & \; 1 + (1+2) + (1+2+4) + (1+2+4+8) & = & \; 26 \\
\end{aligned}
$$

Additionally, per the given problem statement, we also know that

$$A_n = 2^{n + R} + Sn^2 + Tn + U$$

so let's set them equal for $n = 1, 2, 3, 4$:

$$
\begin{aligned}
A_1 & = 1  & = & \; 2^{1 + R} +   S +  T + U & \quad \text{(n = 1)} \quad \text{(1)} \\
A_2 & = 4  & = & \; 2^{2 + R} +  4S + 2T + U & \quad \text{(n = 2)} \quad \text{(2)} \\
A_3 & = 11 & = & \; 2^{3 + R} +  9S + 3T + U & \quad \text{(n = 3)} \quad \text{(3)} \\
A_4 & = 26 & = & \; 2^{4 + R} + 16S + 4T + U & \quad \text{(n = 4)} \quad \text{(4)} \\
\end{aligned}
$$

We now have $4$ equations and $4$ unknowns.

Reorganizing equation $(1)$ to put $R$ on one side, and all the other
variables on the other side, we get:

$$
\begin{aligned}
& 2^{1 + R} +   S +  T + U = 1 & \quad \text{from eq. $1$} \\
& 2^{1 + R} = 1 - S - T - U    & \quad \text{solve for $2^{1+R}$ $(5)$} \\
\end{aligned}
$$

since $2^{1+R}$ appears in all other equations and $R$ does not appear as a
separate variable, we don't have to solve for $R$, and can substitute the
result in $(5)$ into the remaining equations $(2)$, $(3)$, and $(4)$ to remove
the use of variable $R$, leaving us with $3$ equations and $3$ unknowns $(S, T,
U)$.

Let's now take equation $(2)$, separate out $2^{1+R}$ and substitute the result
from $(5)$:

$$
\begin{aligned}
2   \cdot 2^{1 + R} +  4S + 2T + U      & = 4 & \quad \text{from eq. 2} \\
2   \cdot (1 - S - T - U) + 4S + 2T + U & = 4 & \quad \text{substitute from eq. 5} \\
2 - 2S - 2T - 2U + 4S + 2T + U          & = 4 & \quad \text{expand} \\
2 + 2S - U                              & = 4 & \quad \text{simplify} \\
2S - 2                                  & = U & \quad \text{solve for $U$ (6)} \\
\end{aligned}
$$

Now let's take equation $(3)$ and similarly substitute from both $(5)$ and $(6)$:

$$
\begin{aligned}
2^2 \cdot 2^{1 + R} +  9S + 3T + U       & = 11 & \quad \text{from eq. 3} \\
2^2 \cdot (1 - S - T - U) + 9S + 3T + U  & = 11 & \quad \text{substitute $2^{1+R}$ from eq. 5} \\
4 - 4S - 4T - 4U + 9S + 3T + U           & = 11 & \quad \text{expand} \\
5S - T - 3U                              & = 7  & \quad \text{simplify} \\
5S - T - 3(2S - 2)                       & = 7  & \quad \text{substitute $U$ from eq. 6} \\
5S - T - 6S + 6                          & = 7  & \quad \text{expand} \\
-S - T                                   & = 1  & \quad \text{simplify} \\
-S - 1                                   & = T  & \quad \text{solve for $T$ (7)} \\
\end{aligned}
$$

Finally, let's take equation $(4)$ and substitute the results from $(5)$,
$(6)$, and $(7)$ to eliminate all other variables and solve for $S$:

$$
\begin{aligned}
2^3 \cdot 2^{1 + R} + 16S + 4T + U       & = 26 & \quad \text{from eq. 4} \\
2^3 \cdot (1 - S - T - U) + 16S + 4T + U & = 26 & \quad \text{substitute $2^{1+R}$ from eq. 5} \\
8 - 8S - 8T - 8U + 16S + 4T + U          & = 26 & \quad \text{expand} \\
8 + 8S - 4T - 7U                         & = 26 & \quad \text{simplify} \\
8 + 8S - 4(-S - 1) - 7U                  & = 26 & \quad \text{substitute $T$ from eq. 7} \\
8 + 8S - 4(-S - 1) - 7(2S -2)            & = 26 & \quad \text{substitute $U$ from eq. 6} \\
8 + 8S + 4S + 4 - 14S + 14               & = 26 & \quad \text{expand} \\
(8S + 4S - 14S) + (8 + 4 + 14)           & = 26 & \quad \text{combine like terms} \\
-2S + 26                                 & = 26 & \quad \text{simplify} \\
-2S                                      & =  0 & \quad \text{simplify} \\
S                                        & =  0 & \quad \text{solve for $S$ (8)} \\
\end{aligned}
$$

Now that we have $S = 0$, we can go back and substitute this into earlier
equations to find the other unknowns. Let's start with eq. $(7)$ and compute
$T$:

$$ T = -S - 1 = 0 - 1 = -1 $$

Similarly, using eq. $(6)$, we can compute $U$:

$$ U = 2S - 2 = 0 - 2 = - 2 $$

and finally, to compute $R$, we can use eq. $(5)$:

$$
 2^{1 + R} = 1 - S - T - U = 1 - 0 - (-1) - (-2) = 4 = 2^2
$$

Since $2^{1 + R} = 2^2$, we know that $R = 1$. Hence, here are all the unknown
values:

$$
  \boxed{R = 1; \quad S = 0; \quad T = -1; \quad U = -2} \qquad \blacksquare
$$

\textbf{Verification}

Now that we've solved for $R$, $S$, $T$, and $U$, let's verify some of the
$A_n$ values to make sure it works out:

$$
\begin{aligned}
A_1 & = \boxed{ 1} & = & \; 2^{1 + R} +   S +  T + U & = & \; 2^{1 + 1} + 0 - 1 - 2 & = & \; 4  - 3 & = & \; \boxed{ 1} \\
A_2 & = \boxed{ 4} & = & \; 2^{2 + R} +  4S + 2T + U & = & \; 2^{2 + 1} + 0 - 2 - 2 & = & \; 8  - 4 & = & \; \boxed{ 4} \\
A_3 & = \boxed{11} & = & \; 2^{3 + R} +  9S + 3T + U & = & \; 2^{3 + 1} + 0 - 3 - 2 & = & \; 16 - 5 & = & \; \boxed{11} \\
A_4 & = \boxed{26} & = & \; 2^{4 + R} + 16S + 4T + U & = & \; 2^{4 + 1} + 0 - 4 - 2 & = & \; 32 - 6 & = & \; \boxed{26} \\
\end{aligned}
$$

Checks out!
