\textbf{Part (a)}

Use the given equation, substitute, and simplify:

$$
\begin{aligned}
(w \ast x) \ast (y \ast z) & = w \ast z & \quad \text{given} \\
(a \ast b) \ast (a \ast b) & = a \ast b & \quad \text{substitute} \ w = a, x = b, y = a, z = b \\
c \ast c & = c & \quad \text{simplify using} \ a \ast b = c \\
\end{aligned}
$$

This proves that if $a \ast b = c$, then $c \ast c = c$. $\quad \blacksquare$

\textbf{Part (b)}

Use the given equation with some substitutions and utilize the result from part
1:

$$
\begin{aligned}
(w \ast x) \ast (y \ast z) & = w \ast z & \quad \text{given} \\
(c \ast c) \ast (x \ast x) & = c \ast x & \quad \text{substitute} \ w = c, x = c, y = x, z = x \\
c \ast (x \ast x) & = c \ast x & \quad \text{simplify using} \ c \ast c = c \ \text{from part (a)} \\
(a \ast b) \ast (x \ast x) & = c \ast x & \quad \text{expand using} \ a \ast b = c \\
a \ast x & = c \ast x & \quad \text{simplify using given equation} \\
\end{aligned}
$$

This proves that if $a \ast b = c$, then $a \ast x = c \ast x$ for all $x \in S$. $\quad \blacksquare$
